Fix dynamic sealing code, and write specs

theories/examples/dynamic_sealing.v
@@ -18,15 +18,23 @@ Section sealing.
      Result is returned in r_t1; clear r_env for security and return. *)
   (* Arguments: r_t1
      Return point: r_t0
-     Uses: r_env *)
+     Uses: r_env r_t4 (r_t2 rt_3 are used by findb) *)
   Definition unseal_instrs :=
-    encodeInstrsW [ GetB r_t1 r_t1 ]
-                  ++ findb_instr ++
-    encodeInstrsW [ Mov r_env (inl 0%Z)
+    encodeInstrsW [ GetB r_t1 r_t1
+                  ; Mov r_t4 (inr r_t0) (* Save return point *)
+                  ; Mov r_t0 (inr PC) (* Setup the return point for findb *)
+                  ; Lea r_t0 (inl (length findb_instr + 1)%Z)
+                  ; Load r_env r_env (* Need this to use findb_spec ?? *)
+                  ] ++ findb_instr ++
+    encodeInstrsW [ Mov r_env (inl 0%Z) (* Clearing *)
+                  ; Mov r_t0 (inr r_t4) (* Restore return capability *)
+                  ; Mov r_t4 (inl 0%Z) (* Clearing *)
                   ; Jmp r_t0
                   ].
 
   Definition unseal_instrs_length := Eval cbn in length (unseal_instrs).
+  Definition unseal ai :=
+    ([∗ list] a_i;w_i ∈ ai;unseal_instrs, a_i ↦ₐ w_i)%I.
 
   (* Assume r_t1 contains the word to seal.
      Append it to the linked list contained in r_env.
@@ -34,17 +42,24 @@ Section sealing.
      Subseg it, clear r_env and return *)
   (* Arguments: r_t1
      Return point: r_t0
-     Uses: r_env r_t2 *)
+     Uses: r_env r_t2 r_t7 (r_t3 r_t4 r_t5 r_t6 used by appendb) *)
   Definition seal_instrs f_m :=
-    appendb_instr f_m ++
+    encodeInstrsW [ Mov r_t7 (inr r_t0) (* Save return point *)
+                  ; Mov r_t0 (inr PC) (* Setup the return point for findb *)
+                  ; Lea r_t0 (inl (Zlength (appendb_instr f_m)))
+                  ] ++ appendb_instr f_m ++
     encodeInstrsW [ Restrict r_t1 (inl (encodePerm O))
                   ; GetB r_t2 r_t1
                   ; Subseg r_t1 r_t2 r_t2
-                  ; Mov r_env (inl 0%Z)
+                  ; Mov r_env (inl 0%Z) (* Clearing *)
+                  ; Mov r_t0 (inr r_t7) (* Restore return capability *)
+                  ; Mov r_t7 (inl 0%Z) (* Clearing *)
                   ; Jmp r_t0
                   ].
 
   Definition seal_instrs_length := Eval cbn in length (seal_instrs 0%Z).
+  Definition seal f_m ai :=
+    ([∗ list] a_i;w_i ∈ ai;(seal_instrs f_m), a_i ↦ₐ w_i)%I.
 
   (* Create two closures for sealing and unsealing assuming that their code is preceding this one.
      Specifically, we assume the memory layout is [unseal_instrs][seal_instrs][make_seal_preamble] *)
@@ -68,7 +83,7 @@ Section sealing.
                   ]
     ++ crtcls_instrs f_m ++ (* Create the closure for seal, result in r_t1 *)
     encodeInstrsW [ Mov r_t10 r_t1 (* Closure for seal now in r_t10 *)
-                  ; Lea r_t8 (- (Z.of_nat unseal_instrs_length))%Z (* Capability pointing to code for seal_instrs *)
+                  ; Lea r_t8 (inl (- (Z.of_nat unseal_instrs_length))%Z) (* Capability pointing to code for seal_instrs *)
                   ; Mov r_t1 r_t8 (* Prepare for creating closure for unseal, code *)
                   ; Mov r_t1 r_t9 (* Prepare for creating closure for unseal, environment *)
                   ]
@@ -82,5 +97,112 @@ Section sealing.
 
   Definition make_seal_preamble f_m ai :=
     ([∗ list] a_i;w_i ∈ ai;(make_seal_preamble_instrs f_m), a_i ↦ₐ w_i)%I.
+
+  Lemma unseal_spec pc_p pc_b pc_e (* PC *)
+        wret (* return cap *)
+        p b e a (* input cap *)
+        unseal_addrs (* program addresses *)
+        ll ll' (* linked list head and pointers *)
+        a_first a_last (* special adresses *)
+        ι ι1 γ φ (* invariant/gname names *) :
+
+    (* PC assumptions *)
+    isCorrectPC_range pc_p pc_b pc_e a_first a_last ->
+
+    (* Program adresses assumptions *)
+    contiguous_between unseal_addrs a_first a_last ->
+
+    (* linked list ptr element d *)
+    (ll + 1)%a = Some ll' →
+
+    up_close (B:=coPset) ι ⊆ ⊤ ∖ ↑ι1 →
+
+    PC ↦ᵣ inr (pc_p,pc_b,pc_e,a_first)
+      ∗ r_t0 ↦ᵣ wret
+      ∗ r_env ↦ᵣ inr (RWX,ll,ll',ll)
+      ∗ r_t1 ↦ᵣ inr (p, b, e, a)
+      ∗ (∃ w, r_t2 ↦ᵣ w)
+      ∗ (∃ w, r_t3 ↦ᵣ w)
+      ∗ (∃ w, r_t4 ↦ᵣ w)
+      (* invariant for d *)
+      ∗ sealLL ι ll γ
+      (* token which states all non atomic invariants are closed *)
+      ∗ na_own logrel_nais ⊤
+      (* trusted code *)
+      ∗ na_inv logrel_nais ι1 (unseal unseal_addrs)
+      ∗ ▷ φ FailedV
+      ∗ ▷ (PC ↦ᵣ updatePcPerm wret
+          ∗ r_t0 ↦ᵣ wret
+          ∗ r_t2 ↦ᵣ inl 0%Z
+          ∗ (∃ b' w pbvals, ⌜(b + 2)%a = Some b' ∧ (b,w) ∈ pbvals⌝ ∗ prefLL γ pbvals ∗ r_t1 ↦ᵣ w ∗ r_env ↦ᵣ inl 0%Z)
+          ∗ r_t3 ↦ᵣ inl 0%Z
+          ∗ r_t4 ↦ᵣ inl 0%Z
+          ∗ na_own logrel_nais ⊤
+          -∗ WP Seq (Instr Executable) {{ φ }})
+      -∗
+      WP Seq (Instr Executable) {{ φ }}.
+  Proof.
+  Admitted.
+
+  Lemma seal_spec pc_p pc_b pc_e (* PC *)
+        wret (* return cap *)
+        w (* input z *)
+        seal_addrs (* program addresses *)
+        ll ll' pbvals (* linked list head and pointers *)
+        a_first a_last (* special adresses *)
+        rmap (* register map *)
+        f_m b_m e_m (* malloc addrs *)
+        b_r e_r a_r a_r' (* environment table addrs *)
+        ι ι1 ι2 γ Ep φ (* invariant/gname names *) :
+
+    (* PC assumptions *)
+    isCorrectPC_range pc_p pc_b pc_e a_first a_last ->
+
+    (* Program adresses assumptions *)
+    contiguous_between seal_addrs a_first a_last ->
+
+    (* linked list ptr element head *)
+    (ll + 1)%a = Some ll' →
+
+    dom (gset RegName) rmap = all_registers_s ∖ {[ PC; r_env; r_t0; r_t1 ]} →
+
+    (* environment table *)
+    withinBounds (RW, b_r, e_r, a_r') = true →
+    (a_r + f_m)%a = Some a_r' →
+
+    up_close (B:=coPset) ι1 ⊆ Ep →
+    up_close (B:=coPset) ι ⊆ Ep ∖ ↑ι1 →
+    up_close (B:=coPset) ι2 ⊆ Ep ∖ ↑ι1 ∖ ↑ι →
+
+    PC ↦ᵣ inr (pc_p,pc_b,pc_e,a_first)
+       ∗ r_env ↦ᵣ inr (RWX,ll,ll',ll)
+       ∗ r_t1 ↦ᵣ w
+       ∗ r_t0 ↦ᵣ wret
+       ∗ ([∗ map] r↦w ∈ rmap, r ↦ᵣ w)
+       (* own token *)
+       ∗ na_own logrel_nais Ep
+       (* trusted code *)
+       ∗ na_inv logrel_nais ι1 (seal f_m seal_addrs)
+       (* malloc *)
+       ∗ na_inv logrel_nais ι2 (malloc_inv b_m e_m)
+       ∗ pc_b ↦ₐ inr (RO, b_r, e_r, a_r)
+       ∗ a_r' ↦ₐ inr (E, b_m, e_m, b_m)
+       (* linked list invariants *)
+       ∗ sealLL ι ll γ
+       ∗ prefLL γ pbvals
+       ∗ ▷ (PC ↦ᵣ updatePcPerm wret
+          ∗ r_env ↦ᵣ inr (RWX,ll,ll',ll)
+          ∗ r_t0 ↦ᵣ wret
+          ∗ pc_b ↦ₐ inr (RO, b_r, e_r, a_r)
+          ∗ a_r' ↦ₐ inr (E, b_m, e_m, b_m)
+          ∗ ([∗ map] r↦w ∈ <[r_t2:=inl 0%Z]> (<[r_t3:=inl 0%Z]> (<[r_t4:=inl 0%Z]>
+                          (<[r_t5:=inl 0%Z]> (<[r_t6:=inl 0%Z]> (<[r_t7:=inl 0%Z]> rmap))))), r ↦ᵣ w)
+          ∗ (∃ a pbvals', prefLL γ (pbvals ++ pbvals' ++ [(a,w)]) ∗ r_t1 ↦ᵣ inr (RWX,a,a,a))
+          ∗ na_own logrel_nais Ep
+          -∗ WP Seq (Instr Executable) {{ φ }})
+      -∗
+      WP Seq (Instr Executable) {{ λ v, φ v ∨ ⌜v = FailedV⌝ }}.
+  Proof.
+  Admitted.
 
 End sealing.
